parser/Termination.v
@@ -40,60 +40,52 @@ Module TerminationFn (Export D : Defs.T).
 
   (* Termination-related lemmas *)
   
-  Lemma nonzero_exponents_lt_powers_le :
+  Lemma nonzero_exponents_le__powers_le :
     forall b e1 e2,
-      0 < e1 < e2
+      0 < e1 <= e2
       -> b ^ e1 <= b ^ e2.
   Proof.
     intros b e1 e2 [Hlt Hlt']. 
     destruct b as [| b']. 
-    - destruct e1; destruct e2; auto.
-      omega.
-    - destruct b' as [| b''].
-      + repeat rewrite Nat.pow_1_l; auto.
-      + pose proof Nat.pow_lt_mono_r as H. 
-        specialize (H (S (S b'')) e1 e2). 
-        assert (fact : forall n m, n < m -> n <= m) by (intros; omega).
-        apply fact.
-        apply Nat.pow_lt_mono_r; auto.
-        omega.
+    - destruct e1; destruct e2; auto; omega.
+    - apply Nat.pow_le_mono_r; auto. 
   Qed.
   
-  Lemma nonzero_exponents_lt_tailFrameScore_le :
+  Lemma nonzero_exponents_le__tailFrameScore_le :
     forall fr b e1 e2,
-      0 < e1 < e2
+      0 < e1 <= e2
       -> tailFrameScore fr b e1 <= tailFrameScore fr b e2.
   Proof.
     intros fr b e1 e2 Hlt.
     unfold tailFrameScore. 
     apply Nat.mul_le_mono_l.
-    apply nonzero_exponents_lt_powers_le; auto.
+    apply nonzero_exponents_le__powers_le; auto.
   Qed.
 
-  Lemma nonzero_exponents_lt_tailFramesScore_le :
+  Lemma nonzero_exponents_le__tailFramesScore_le :
     forall frs b e1 e2,
-      0 < e1 < e2
+      0 < e1 <= e2
       -> tailFramesScore frs b e1 <= tailFramesScore frs b e2.
   Proof.
     intros frs.
     induction frs as [| fr frs' IH]; intros b e1 e2 Hlt; simpl; auto.
     apply plus_le_compat.
-    - apply nonzero_exponents_lt_tailFrameScore_le; auto.
+    - apply nonzero_exponents_le__tailFrameScore_le; auto.
     - apply IH; omega.
   Qed.
 
-  Lemma nonzero_exponents_lt_stackScore_le :
+  Lemma nonzero_exponents_le__stackScore_le :
     forall v b e1 e2 e3 e4 frs,
-      0 < e1 < e2
-      -> 0 < e3 < e4
+      0 < e1 <= e2
+      -> 0 < e3 <= e4
       -> v * (b ^ e1) + tailFramesScore frs b e3 <= 
          v * (b ^ e2) + tailFramesScore frs b e4.
   Proof.
     intros v b e1 e2 e3 e4 frs [H0e1 He1e2] [H0e3 He3e4].
     apply plus_le_compat.
     - apply Nat.mul_le_mono_l. 
-      apply nonzero_exponents_lt_powers_le; auto.
-    - apply nonzero_exponents_lt_tailFramesScore_le; auto.
+      apply nonzero_exponents_le__powers_le; auto.
+    - apply nonzero_exponents_le__tailFramesScore_le; auto.
   Qed.
 
   Lemma mem_true_cardinality_neq_0 :
@@ -115,37 +107,110 @@ Module TerminationFn (Export D : Defs.T).
     apply mem_true_cardinality_neq_0 in Hm; omega.
   Qed.
 
-  Lemma stackScore_le_after_return :
-    forall callee caller caller' o o' x x' suf' av locs b,
-      callee = SF o []
-      -> caller  = SF o' (NT x' :: suf')
-      -> caller' = SF o' suf'
-      -> stackScore (caller', locs) b (NtSet.cardinal (NtSet.add x av))
-         <= stackScore (callee, caller :: locs) b (NtSet.cardinal av).
+  Lemma cardinal_diff_remove_gt_0 :
+    forall x s s',
+      NtSet.In x s
+      -> 0 < NtSet.cardinal (NtSet.diff s (NtSet.remove x s')).
   Proof.
-    intros ce cr cr' o o' x x' suf' av locs b hce hcr hcr'; subst.
+    intros x s s' hm.
+    apply mem_true_cardinality_gt_0 with (x := x).
+    apply NF.mem_iff; ND.fsetdec.
+  Qed.
+
+  Lemma cardinal_diff_gt_0 :
+    forall x s s',
+      NtSet.In x s
+      -> ~ NtSet.In x s'
+      -> 0 < NtSet.cardinal (NtSet.diff s s').
+  Proof.
+    intros x s s' hi hn.
+    apply mem_true_cardinality_gt_0 with (x := x).
+    apply NF.mem_iff; ND.fsetdec.
+  Qed.
+
+  Lemma diff_remove_equal_add_diff :
+    forall x s s',
+      NtSet.In x s
+      -> NtSet.Equal (NtSet.diff s (NtSet.remove x s'))
+                     (NtSet.add x (NtSet.diff s s')).
+  Proof.
+    intros; ND.fsetdec.
+  Qed.
+
+  Lemma diff_remove_equal_diff_1 :
+    forall x s s',
+      ~ NtSet.In x s
+      -> NtSet.Equal (NtSet.diff s (NtSet.remove x s')) (NtSet.diff s s').
+  Proof.
+    intros x s s' hm; ND.fsetdec.
+  Qed.
+  
+  Lemma diff_remove_equal_diff_2 :
+    forall x s s',
+      ~ NtSet.In x s'
+      -> NtSet.Equal (NtSet.diff s (NtSet.remove x s')) (NtSet.diff s s').
+  Proof.
+    intros x s s' hm; ND.fsetdec.
+  Qed.
+  
+  Lemma cardinal_diff_remove_le :
+    forall x s s',
+      NtSet.In x s
+      -> NtSet.In x s'
+      -> NtSet.cardinal (NtSet.diff s (NtSet.remove x s')) <=
+         S (NtSet.cardinal (NtSet.diff s s')).
+    intros x s s' hi hm.
+    rewrite diff_remove_equal_add_diff; auto.
+    rewrite add_cardinal_2; auto.
+    apply not_mem_iff; ND.fsetdec.
+  Qed.
+
+  Lemma diff_remove_equal_diff :
+    forall x s s',
+      ~ NtSet.In x s
+      -> NtSet.Equal (NtSet.diff s (NtSet.remove x s'))
+                     (NtSet.diff s s').
+  Proof.
+    intros; ND.fsetdec.
+  Qed.
+  
+  Lemma stackScore_le_after_return :
+    forall callee caller caller' o o' x suf vi u locs b,
+      callee     = SF o' []
+      -> caller  = SF o (NT x :: suf)
+      -> caller' = SF o suf
+      -> NtSet.In x u
+      -> stackScore (caller', locs) b (NtSet.cardinal (NtSet.diff u (NtSet.remove x vi)))
+         <= stackScore (callee, caller :: locs) b (NtSet.cardinal (NtSet.diff u vi)).
+  Proof.
+    intros ce cr cr' o o' x suf vi u locs b hce hcr hcr' hi; subst.
     unfold stackScore; simpl.
     unfold headFrameScore; unfold headFrameSize.
     unfold tailFrameScore; unfold tailFrameSize.
-    destruct (NtSet.mem x av) eqn:hm.
-    - rewrite add_cardinal_1; auto.
-      eapply nonzero_exponents_lt_stackScore_le.
-      + split; auto.
-        eapply mem_true_cardinality_gt_0; eauto.
-      + split; omega.
-    - rewrite add_cardinal_2; auto.
-  Qed.
+    destruct (NtSet.mem x vi) eqn:hm.
+    - apply NF.mem_iff in hm.
+      assert (hi' : NtSet.In x u) by ND.fsetdec.
+      apply nonzero_exponents_le__stackScore_le; split; try omega.
+      + apply cardinal_diff_remove_gt_0; auto. 
+      + apply cardinal_diff_remove_le; auto.
+      + apply le_n_S; apply cardinal_diff_remove_le; auto. 
+    - apply not_mem_iff in hm.
+      rewrite diff_remove_equal_diff_2; auto.
+      apply nonzero_exponents_le__stackScore_le; split; try omega.
+      eapply cardinal_diff_gt_0; eauto.
+  Qed.      
 
   (* this version might be easier to apply *)
   Lemma stackScore_le_after_return' :
-    forall suf_cr o o' x b av frs,
-      stackScore (SF o' suf_cr, frs) 
-                 b 
-                 (NtSet.cardinal (NtSet.add x av))
-      <= 
-      stackScore (SF o [], SF o' (NT x :: suf_cr) :: frs) 
-                 b 
-                 (NtSet.cardinal av).
+    forall suf_cr o o' x b vi u frs,
+      NtSet.In x u 
+      -> stackScore (SF o suf_cr, frs) 
+                    b 
+                    (NtSet.cardinal (NtSet.diff u (NtSet.remove x vi)))
+         <= 
+         stackScore (SF o' [], SF o (NT x :: suf_cr) :: frs) 
+                    b 
+                    (NtSet.cardinal (NtSet.diff u vi)).
   Proof.
     intros; eapply stackScore_le_after_return; sis; eauto.
   Qed.
@@ -200,44 +265,65 @@ Module TerminationFn (Export D : Defs.T).
       apply IH; omega. 
   Qed.
 
+  Lemma diff_add_equal_remove_diff :
+    forall x s s',
+      NtSet.Equal (NtSet.diff s (NtSet.add x s'))
+                  (NtSet.remove x (NtSet.diff s s')).
+  Proof.
+    intros x s s'; ND.fsetdec.
+  Qed.
+
+  Lemma cardinal_diff_minus_1 :
+    forall x s s',
+      NtSet.In x s
+      -> ~ NtSet.In x s'
+      -> S (NtSet.cardinal (NtSet.diff s (NtSet.add x s'))) =
+         NtSet.cardinal (NtSet.diff s s').
+  Proof.
+    intros x s s' hi hn.
+    rewrite diff_add_equal_remove_diff.
+    apply remove_cardinal_1.
+    apply NF.mem_iff; ND.fsetdec.
+  Qed.
+  
   Lemma stackScore_lt_after_push :
-    forall g callee caller o o' x suf' av rhs locs,
-      callee = SF o rhs
+    forall pm callee caller o o' x suf' u vi rhs locs,
+      callee    = SF o rhs
       -> caller = SF o' (NT x :: suf')
-      -> NtSet.In x av
-      -> In (x, rhs) g
+      -> NtSet.In x u
+      -> ~ NtSet.In x vi
+      -> In (x, rhs) (grammarOf pm)
       -> stackScore (callee, caller :: locs)
-                    (1 + maxRhsLength g)
-                    (NtSet.cardinal (NtSet.remove x av))
+                    (1 + maxRhsLength (grammarOf pm))
+                    (NtSet.cardinal (NtSet.diff u (NtSet.add x vi)))
          <
          stackScore (caller, locs)
-                    (1 + maxRhsLength g)
-                    (NtSet.cardinal av).
+                    (1 + maxRhsLength (grammarOf pm))
+                    (NtSet.cardinal (NtSet.diff u vi)).
   Proof.
-    intros g callee caller o o' x suf' av rhs locs
-           Hcallee Hcaller Hin Hin'; subst; simpl.
-    apply NF.mem_iff in Hin.
-    rewrite remove_cardinal_1; auto.
+    intros pm callee caller o o' x suf' u vi rhs locs
+           Hcallee Hcaller Hin Hnin Hi'; subst; simpl.
+    rewrite cardinal_diff_minus_1; auto.
     unfold headFrameScore; unfold headFrameSize.
     unfold tailFrameScore; unfold tailFrameSize; simpl.
-    rewrite plus_assoc; repeat apply plus_lt_compat_r.
-    rewrite remove_cardinal_minus_1; auto.
+    repeat rewrite plus_assoc; repeat apply plus_lt_compat_r.
     apply less_significant_value_lt_more_significant_digit.
     - eapply grammar_rhs_length_lt_max_plus_1; eauto.
-    - erewrite <- remove_cardinal_1; eauto; omega.
+    - apply subset_cardinal_lt with (x := x); ND.fsetdec. 
   Qed.
 
   Lemma stackScore_lt_after_push' :
-    forall g suf_cr rhs o o' x av locs,
-      NtSet.In x av
-      -> In (x, rhs) g
+    forall pm suf_cr rhs o o' x u vi locs,
+      NtSet.In x u
+      -> ~ NtSet.In x vi
+      -> In (x, rhs) (grammarOf pm)
       -> stackScore (SF o rhs, SF o' (NT x :: suf_cr) :: locs)
-                    (1 + maxRhsLength g)
-                    (NtSet.cardinal (NtSet.remove x av))
+                    (1 + maxRhsLength (grammarOf pm))
+                    (NtSet.cardinal (NtSet.diff u (NtSet.add x vi)))
          <
          stackScore (SF o' (NT x :: suf_cr), locs)
-                    (1 + maxRhsLength g)
-                    (NtSet.cardinal av).
+                    (1 + maxRhsLength (grammarOf pm))
+                    (NtSet.cardinal (NtSet.diff u vi)).
   Proof.
     intros; eapply stackScore_lt_after_push; sis; eauto.
   Qed.
